Impl/BucketIteratorModel.i.dfy
@@ -2,8 +2,7 @@ include "../PivotBetree/BucketsLib.i.dfy"
 include "../lib/Base/Sets.i.dfy"
 //
 // A mathematical description of bucket iterators.
-// This model is used directly as the iterator for BucketImpl,
-// hence there is no corresponding BucketIteratorImpl class.
+// The implementation is defined in BucketImpl together with MutBucket.
 //
 
 module BucketIteratorModel {
