lib/DataStructures/PackedStringArray.i.dfy
@@ -125,7 +125,7 @@ module PackedStringArray {
 
   lemma lemma_seq_slice_suffix<T>(s: seq<T>, i: int, j: int, k: int)
   requires 0 <= i <= j <= |s|
-  requires k <= j - i
+  requires 0 <= k <= j - i
   ensures s[i..j][k..] == s[i+k..j];
   {
   }
